chapter04/demos/leader_election_instructor_script.md
@@ -43,7 +43,6 @@ so instead of teaching you how to manage mod, let's just bail on it.
 So time to dig into the broken proof.
 * Choose a step. (get through the exists, skolemize the step choice & params)
 
-XXX does the inductive invariant lesson preced this one?
 ...wait, why would this even work? Safety is like the manhole: a good property, but not
 inductive. Lots of system states that are a step away from Safety but shouldn't be
 reachable.
@@ -90,7 +89,7 @@ Cheat sheet:
 ```
 
 Proof sketch:
-If we are gonna violate Safety, we'll need two idxes i, j that both think they're
+If we are gonna violate Safety, we'll need two idxes i, j tha
 leader. WOLOG let i be the one with the larger id. It is leader, so IsChord(k,v,i,i).
 So every *other* node, including j is Between(k, i, j, i), so
 v.highest_heard[j] > k.ids[j], which is a contradiction with IsLeader(j).
@@ -123,7 +122,127 @@ Use a case analysis on dst
 ...now the proof goes through.
 
 
-***
+*** TODO -- XXX
 Image fixes:
 - dafny-profile.py
 - pip3 install termcolor
+***
+
+
+------------------------------------------------------------------------------
+
+# Another run-through.
+
+Fresh file. Run Dafny.
+* "value does not satisfy the subset constraints..."
+* fix those three, then a timeout!?
+```
+../../tools/dafny-profile.py 20 "*NextPreservesInv" leader_election_work.dfy 
+```
+No quantifiers instantiated more than 1000 times.
+
+* try noNLarith
+dafny leader_election_work.dfy /noNLarith
+Fails fast
+
+nlarith lecture
+
+```
+  if idx+1 == |k.ids| then 0 else idx+1
+```
+
+XXX does the inductive invariant lesson preced this one?
+
+# Define invariant
+
+...wait, why would this even work? Safety is like the manhole: a good property, but not
+inductive. Lots of system states that are a step away from Safety but shouldn't be
+reachable.
+It's time to ask *why* should the system work? What's the key intuition?
+The answer is in the animation: As "big" identifiers work around the ring, they
+build "chords" from their origin to the farthest point they've reached.
+Sometimes one chord will gobble up another's head, breaking it, but anytime there is a
+chord, all the nodes it has passed over have heard about it and are dominated by it.
+The biggest ID's chord never gets gobbled; eventually it reaches all the way around the ring.
+
+Type out IsChord, OnChordHeardDominatesId.
+
+Cheat sheet:
+```
+  predicate Between(start: nat, i: nat, end: nat)
+  {
+    if start<end
+    then start<i<end
+    else i<end || start<i
+  }
+
+  predicate IsChord(k: Constants, v: Variables, start: nat, end: nat)
+  {
+    && k.WF()
+    && v.WF(k)
+    && k.ValidIdx(start)
+    && k.ValidIdx(end)
+    && k.ids[start] == v.highest_heard[end]
+  }
+
+  predicate OnChordHeardDominatesId(k: Constants, v: Variables, start: nat, end: nat)
+    requires k.WF()
+    requires v.WF(k)
+  {
+    forall i:nat | k.ValidIdx(i) && Between(start, i, end) :: v.highest_heard[i] > k.ids[i]
+  }
+
+  predicate OnChordHeardDominatesIdInv(k: Constants, v: Variables)
+    requires k.WF()
+    requires v.WF(k)
+  {
+    forall start:nat, end:nat | k.ValidIdx(start) && k.ValidIdx(end) && IsChord(k, v, start, end) :: OnChordHeardDominatesId(k, v, start, end)
+  }
+```
+
+Proof sketch:
+If we are gonna violate Safety, we'll need two idxes i, j tha
+leader. WOLOG let i be the one with the larger id. It is leader, so IsChord(k,v,i,i).
+So every *other* node, including j is Between(k, i, j, i), so
+v.highest_heard[j] > k.ids[j], which is a contradiction with IsLeader(j).
+
+...need to define Between.
+
+* bring assert into NextPreservesInv
+
+* introduce variables.
+  :| for step,
+  forall-statement for {start,end}, i
+
+* split on dst==end, ...
+
+* split dst==end on 
+        if v'.highest_heard[dst] == v.highest_heard[dst] {
+        } else if v'.highest_heard[dst] == k.ids[src] {
+        } else {
+          assert v'.highest_heard[dst] == v.highest_heard[src];
+        }
+        ...fails middle branch
+
+* middle branch:
+          assert k.ids[src] > v.highest_heard[dst];
+
+  WHAT? Assert some true stuff
+          assert v'.highest_heard[dst] == dst_new_max;
+          assert dst_new_max != v.highest_heard[src];
+          assert dst_new_max == message;
+          assert message > v.highest_heard[dst];
+   ...dst_new_max fails!?
+          
+  look at defn.
+  FIX dst_new_max
+
+* okay, still on dst==end and v'.highest_heard[dst] == k.ids[src]
+  In this case, we have a little chord from src->dst, but also a chord
+  from start->dst.
+  So k.ids[src] == k.ids[start];
+  That's fine if src==start, but that would exclude
+  Between(start, i, dst).
+  So src!=start.
+  assert k.UniqueIds()!
+  FIX UniqueIds.
